<?xml version="1.0" encoding="utf-8"?>
<rdf:RDF
   xmlns:bio="http://purl.org/vocab/bio/0.1/"
   xmlns:dcterms="http://purl.org/dc/terms/"
   xmlns:foaf="http://xmlns.com/foaf/0.1/"
   xmlns:owl="http://www.w3.org/2002/07/owl#"
   xmlns:rdf="http://www.w3.org/1999/02/22-rdf-syntax-ns#"
   xmlns:rdfs="http://www.w3.org/2000/01/rdf-schema#"
   xmlns:skos="http://www.w3.org/2004/02/skos/core#"
   xmlns="http://poderopedia.com/vocab/">
  <rdf:Description rdf:about="http://poderopedia.com/vocab/AcademicConnection">
    <rdfs:comment xml:lang="es">La relación entre una persona y una organización académica (colegio, universidad, etc)</rdfs:comment>
    <rdfs:comment xml:lang="en">The connection between a person and an Educational Organization (university, school, etc)</rdfs:comment>
    <rdfs:label xml:lang="en">Academic Connection</rdfs:label>
    <rdfs:label xml:lang="es">Conexión académica</rdfs:label>
    <rdfs:subClassOf rdf:resource="http://purl.org/vocab/bio/0.1/Relationship"/>
  </rdf:Description>
  <rdf:Description rdf:about="http://poderopedia.com/vocab/BelongingConnection">
    <rdfs:comment xml:lang="es">La relación entre una persona y una organización (Opus Dei, un Think Tank) sin necesariamente estar afiliado</rdfs:comment>
    <rdfs:comment xml:lang="en">The connection between a person and a Organization (Opus Dei, a Think Tank) without been affiliated to it necessarily</rdfs:comment>
    <rdfs:label xml:lang="en">Belonging Connection</rdfs:label>
    <rdfs:label xml:lang="es">Conexión de pertenencia</rdfs:label>
    <rdfs:subClassOf rdf:resource="http://purl.org/vocab/bio/0.1/Relationship"/>
  </rdf:Description>
  <owl:Class rdf:about="http://poderopedia.com/vocab/Company">
    <rdfs:comment>A for profit organization</rdfs:comment>
    <rdfs:label>Company</rdfs:label>
    <rdfs:subClassOf rdf:resource="http://xmlns.com/foaf/0.1/Agent"/>
    <owl:disjointWith rdf:resource="http://poderopedia.com/vocab/Organization"/>
    <owl:disjointWith rdf:resource="http://xmlns.com/foaf/0.1/Person"/>
  </owl:Class>
  <rdf:Description rdf:about="http://poderopedia.com/vocab/EconomicConnection">
    <rdfs:comment xml:lang="es">La relación entre una persona y una organización académica (colegio, universidad, etc)</rdfs:comment>
    <rdfs:comment xml:lang="en">The connection between a person and an Educational Organization (university, school, etc)</rdfs:comment>
    <rdfs:label xml:lang="es">Conexión económica</rdfs:label>
    <rdfs:label xml:lang="en">Economic Connection</rdfs:label>
    <rdfs:subClassOf rdf:resource="http://purl.org/vocab/bio/0.1/Relationship"/>
  </rdf:Description>
  <owl:Class rdf:about="http://poderopedia.com/vocab/Organization">
    <rdfs:comment>An organization that is not a company</rdfs:comment>
    <rdfs:label>Organization</rdfs:label>
    <rdfs:subClassOf rdf:resource="http://xmlns.com/foaf/0.1/Agent"/>
    <owl:disjointWith rdf:resource="http://poderopedia.com/vocab/Company"/>
    <owl:disjointWith rdf:resource="http://xmlns.com/foaf/0.1/Person"/>
  </owl:Class>
  <rdf:Property rdf:about="http://poderopedia.com/vocab/academicOrganizationParticipant">
    <rdf:type rdf:resource="http://www.w3.org/2002/07/owl#ObjectProperty"/>
    <rdfs:comment xml:lang="es">Indica qué organización académica está asociada a una conección académica en particular</rdfs:comment>
    <rdfs:comment xml:lang="en">Indicates which academic organization is associated in a particular academic connection</rdfs:comment>
    <rdfs:domain rdf:resource="http://poderopedia.com/vocab/AcademicConnection"/>
    <rdfs:label xml:lang="en">Academic organization</rdfs:label>
    <rdfs:label xml:lang="es">Organización académica</rdfs:label>
    <rdfs:range rdf:resource="http://poderopedia.com/vocab/Organization"/>
    <rdfs:subClassOf rdf:resource="http://purl.org/vocab/bio/0.1/participant"/>
  </rdf:Property>
  <rdf:Property rdf:about="http://poderopedia.com/vocab/alias">
    <rdf:type rdf:resource="http://www.w3.org/2002/07/owl#DatatypeProperty"/>
    <rdfs:domain rdf:resource="http://xmlns.com/foaf/0.1/Person"/>
    <rdfs:label xml:lang="en">An alias for a person</rdfs:label>
    <rdfs:label xml:lang="es">Segundo apellido</rdfs:label>
    <rdfs:subPropertyOf rdf:resource="http://www.w3.org/2004/02/skos/core#altLabel"/>
    <rdfs:subPropertyOf rdf:resource="http://xmlns.com/foaf/0.1/name"/>
  </rdf:Property>
  <rdf:Property rdf:about="http://poderopedia.com/vocab/firstLastName">
    <rdf:type rdf:resource="http://www.w3.org/2002/07/owl#DatatypeProperty"/>
    <rdfs:domain rdf:resource="http://xmlns.com/foaf/0.1/Person"/>
    <rdfs:label xml:lang="en">First last name</rdfs:label>
    <rdfs:label xml:lang="es">Primer apellido</rdfs:label>
    <rdfs:subPropertyOf rdf:resource="http://xmlns.com/foaf/0.1/familyName"/>
  </rdf:Property>
  <rdf:Property rdf:about="http://poderopedia.com/vocab/secondLastName">
    <rdf:type rdf:resource="http://www.w3.org/2002/07/owl#DatatypeProperty"/>
    <rdfs:domain rdf:resource="http://xmlns.com/foaf/0.1/Person"/>
    <rdfs:label xml:lang="en">Second last name</rdfs:label>
    <rdfs:label xml:lang="es">Segundo apellido</rdfs:label>
    <rdfs:subPropertyOf rdf:resource="http://xmlns.com/foaf/0.1/familyName"/>
  </rdf:Property>
  <owl:Class rdf:about="http://xmlns.com/foaf/0.1/Person"/>
</rdf:RDF>
