@prefix rdf:      <http://www.w3.org/1999/02/22-rdf-syntax-ns#> .
@prefix owl:      <http://www.w3.org/2002/07/owl#> .
@prefix skos:     <http://www.w3.org/2004/02/skos/core#> .
@prefix bio:      <http://purl.org/vocab/bio/0.1/> .
@prefix rel:      <http://purl.org/vocab/relationship/> .
@prefix foaf:     <http://xmlns.com/foaf/0.1/> .
@prefix rdfs:     <http://www.w3.org/2000/01/rdf-schema#> .
@prefix dcterms:  <http://purl.org/dc/terms/> .
@prefix label: <http://purl.org/net/vocab/2004/03/label#> .
@prefix vann: <http://purl.org/vocab/vann/> .
@prefix xsd: <http://www.w3.org/2001/XMLSchema#> .
@prefix :         <http://poderopedia.com/vocab/> .



:schema rdf:type owl:Ontology ;
        dcterms:title "PoderVocab: A vocabulary for Poderopedia"@en, "PoderVocab: Un vocabulario para Poderopedia"@es ;
        dcterms:date "2012-03-30"^^xsd:date ;
        dcterms:abstract "This document describes a vocabulary to express information about people and their relations with Organizations, Companies, etc."@en,
                         "Este documento describe un vocabulario para expresar información acerca de personas, y sus relaciones con organizaciones y empresas"@es;
        owl:imports <http://purl.org/vocab/bio/0.1/>.
        
        
##Entities

# People
foaf:Person a owl:Class.

# Relations for foaf:Person

                    
:firstLastName a rdf:Property, owl:DatatypeProperty;
               rdfs:subPropertyOf foaf:familyName;
               rdfs:label "First last name"@en, "Primer apellido"@es;
               rdfs:domain foaf:Person ;
               rdfs:range rdfs:Literal .
               
:secondLastName a rdf:Property, owl:DatatypeProperty;
                rdfs:subPropertyOf foaf:familyName;
                rdfs:label "Second last name"@en, "Segundo apellido"@es;
                rdfs:domain foaf:Person ;
                rdfs:range rdfs:Literal .

:alias a rdf:Property, owl:DatatypeProperty;
         rdfs:subPropertyOf foaf:name, skos:altLabel;
         rdfs:label "An alias for a person"@en, "Segundo apellido"@es;
         rdfs:domain foaf:Person ;
         rdfs:range rdfs:Literal .

         
# Companies

:Company a owl:Class;
         rdfs:subClassOf  foaf:Agent;
         rdfs:label       "Company";
         rdfs:comment     "A for profit organization";
         owl:disjointWith foaf:Person, :Organization.

## EconomicConnection
:EconomicConnection rdfs:subClassOf bio:Relationship;
                    rdfs:label "Economic Connection"@en, "Conexión económica"@es;
                    rdfs:comment "The connection between a person and an Educational Organization (university, school, etc)"@en, "La relación entre una persona y una organización académica (colegio, universidad, etc)"@es.              

                                 
### EconomicConnection relations
:companyParticipant a rdf:Property, owl:ObjectProperty;
                    rdfs:subPropertyOf bio:participant;
                    rdfs:label "Company related"@en, "Empresa relacionada"@es;
                    rdfs:comment "Indicates which company is associated in a particular economic connection"@en, "Indica qué empresa está asociada en una conección económica"@es;
                    rdfs:domain :EconomicConnection;
                    rdfs:range :Company.                      

:declarationOfPatrimony a rdf:Property, owl:ObjectProperty;
                        rdfs:label "Declaration of Patrimony"@en, "Declaración de Patrimonio"@es;
                        rdfs:domain :EconomicConnection;
                        rdfs:range rdfs:Resource.
                        
:declarationOfInterests a rdf:Property, owl:ObjectProperty;
                        rdfs:label "Declaration of interests"@en, "Declaración de intereses"@es;
                        rdfs:domain :EconomicConnection;
                        rdfs:range rdfs:Resource.
                        
                                                
# Organizations

:Organization a owl:Class;
              rdfs:subClassOf  foaf:Agent;
              rdfs:label       "Organization";
              rdfs:comment     "An organization that is not a company";
              owl:disjointWith foaf:Person, :Company.
         

                
:AcademicConnection a rdfs:Class;
                    rdfs:subClassOf bio:Relationship;
                    rdfs:label "Academic Connection"@en, "Conexión académica"@es;
                    rdfs:comment "The connection between a person and an Educational Organization (university, school, etc)"@en, "La relación entre una persona y una organización académica (colegio, universidad, etc)"@es.
                                 
:BelongingConnection rdfs:subClassOf bio:Relationship;
                     rdfs:label "Belonging Connection"@en, "Conexión de pertenencia"@es;
                     rdfs:comment "The connection between a person and a Organization (Opus Dei, a Think Tank) without been affiliated to it necessarily"@en, "La relación entre una persona y una organización (Opus Dei, un Think Tank) sin necesariamente estar afiliado"@es.              
                    
                     
                     
                     
## AcademicConnection relations                     
:academicOrganizationParticipant a rdf:Property, owl:ObjectProperty;
                                 rdfs:subClassOf bio:participant;
                                 rdfs:label "Academic organization"@en, "Organización académica"@es;
                                 rdfs:comment "Indicates which academic organization is associated in a particular academic connection"@en, "Indica qué organización académica está asociada a una conección académica en particular"@es;
                                 rdfs:domain :AcademicConnection;
                                 rdfs:range :Organization.

                      
:partnerParticipant a rdf:Property, owl:ObjectProperty;
                    rdfs:subPropertyOf bio:participant;
                    rdfs:label "Partner related"@en, "Persona asociada"@es;
                    rdfs:comment "Relates a person to a particular economic connection"@en, "Relaciona a una persona en una conección económica"@es;
                    rdfs:domain :EconomicConnection;
                    rdfs:range foaf:Person.                        

                
##NewsEvent

:NewsEvent a rdfs:Class;
           rdfs:subClassOf bio:Event;
           rdfs:label "News event"@en, "Evento noticioso"@es;
           rdfs:comment "An event relevant from the point of view of journalism"@en, "Un evento de relevancia periodística"@es.
           
:NewsEventConnection a rdfs:Class;
                     rdfs:subClassOf bio:Relationship;
                     rdfs:label "News event connection"@en, "Conección con evento noticioso"@es;
                     rdfs:comment "Describes the relation of a person with a news event during a specific period of time"@en, "Describe la relación de una persona con un evento noticioso durante un período de tiempo"@es.
                     
:newsEventParticipant a rdf:Property;
                      rdfs:subPropertyOf bio:participant;
                      rdfs:domain :NewsEventConnection;
                      rdfs:range foaf:Person;
                      rdfs:label "News event participant".
                      
:newsEventRelated a rdf:Property;
                  rdfs:subPropertyOf bio:participant;
                  rdfs:domain :NewsEventConnection;
                  rdfs:range :NewsEvent;
                  rdfs:label "News event associated".                      
                      
                      
                      
                      
                      
                      
                      
                      
                      
                      
                      
                      
                      
                      
                      
                      
#
bio:participant owl:equivalentProperty rel:participant ;
                                            rdfs:comment "A person, group or organization that participates in a relationship for some time."@en ;
                                            rdfs:subPropertyOf <http://www.w3.org/2002/07/owl#differentFrom> ;
                                            rdfs:domain <http://purl.org/vocab/bio/0.1/Relationship> ;
                                            owl:inverseOf <http://purl.org/vocab/bio/0.1/relationship> ;
                                            rdf:type rdf:Property, owl:ObjectProperty ;
                                            dcterms:issued "2011-06-14" ;
                                            rdfs:range <http://xmlns.com/foaf/0.1/Agent> ;
                                            rdfs:isDefinedBy <http://purl.org/vocab/bio/0.1/> ;
                                            label:plural "Participants"@en ;
                                            rdfs:label "Participant"@en .

                                            
bio:Event rdfs:subClassOf <http://purl.org/NET/c4dm/event.owl#Event> ,
                                                     <http://linkedevents.org/ontology/Event> ,
                                                     <http://purl.org/dc/dcmitype/Event> ,
                                                     <http://sw.opencyc.org/2009/04/07/concept/en/Event> ;
                                      rdf:type owl:Class ;
                                      rdfs:isDefinedBy <http://purl.org/vocab/bio/0.1/> ;
                                      rdfs:label "Event"@en ;
                                      rdfs:comment "An event is an occurrence that brings about a change in the state of affairs for one or more people and/or other agents. Events are assumed to occur over a period of time and may not have precise start and end points."@en ;
                                      vann:usageNote "This class is intended to describe biographical events, i.e. events in the life of a person."@en .

bio:concludingEvent
    dcterms:issued "2010-05-06" ;
    <http://purl.org/net/vocab/2004/03/label#plural> "Concluding Event"@en ;
    a rdf:Property, <http://www.w3.org/2002/07/owl#ObjectProperty> ;
    rdfs:comment "An event that marks the end of an interval and/or relationship. The event changes of the state of affairs that held during the interval. For example a period of study may be concluded by a Graduation event."@en ;
    rdfs:isDefinedBy <http://purl.org/vocab/bio/0.1/> ;
    rdfs:label "Concluding Event"@en ;
    rdfs:range bio:Event ;
    rdfs:subPropertyOf owl:differentFrom .
    
    
bio:initiatingEvent
    dcterms:issued "2010-05-06" ;
    <http://purl.org/net/vocab/2004/03/label#plural> "Initiating Event"@en ;
    a rdf:Property, owl:ObjectProperty ;
    rdfs:comment "An event that marks the start of an interval and/or relationship. The event contributes to and/or causes of the state of affairs that hold during the interval. For example a period of study may be initiated by an Enrolment event."@en ;
    rdfs:isDefinedBy <http://purl.org/vocab/bio/0.1/> ;
    rdfs:label "Initiating Event"@en ;
    rdfs:range bio:Event ;
    rdfs:subPropertyOf owl:differentFrom .    
